Add 'Add' primitive

pure_langScript.sml
@@ -17,6 +17,7 @@ Datatype:
      | Cons string      (* datatype constructor             *)
      | IsEq string      (* compare cons tag                 *)
      | Proj string num  (* reading a field of a constructor *)
+     | Add              (* primitive add operator           *)
 End
 
 Datatype:
@@ -131,6 +132,12 @@ Definition is_eq_def:
       | _ => Error
 End
 
+
+Definition getNum_def:
+  getNum (Num n) = SOME n ∧
+  getNum _       = NONE
+End
+
 Definition eval_op_def:
   (eval_op (Lit n) [] = Num n) ∧
   (eval_op (Cons s) xs = Constructor s xs) ∧
@@ -140,6 +147,12 @@ Definition eval_op_def:
     if x1 = Num 0 then x3 else Error) ∧
   (eval_op (IsEq s) [x] = is_eq s x) ∧
   (eval_op (Proj s i) [x] = el s i x) ∧
+  (eval_op Add [a1;a2] =
+     if a1 = Diverge then Diverge else
+     if a2 = Diverge then Diverge else
+   case (getNum a1,getNum a2) of
+     | (SOME n1,SOME n2) => (Num (n1 + n2))
+     | _               => Error )  ∧
   (eval_op _ _ = Error)
 End
 
@@ -390,6 +403,58 @@ Proof
   \\ Cases_on ‘y’ \\ fs []
 QED
 
+Theorem getNum_eq_same_length_args:
+  ∀ ts ts' . LLENGTH ts = LLENGTH ts'
+             ⇒ getNum (Branch q ts) = getNum (Branch q ts')
+Proof
+  Cases_on ‘q’ \\ Cases_on ‘ts’ \\ Cases_on ‘ts'’ \\ rw [getNum_def]
+QED
+
+Theorem v_cmp_getNum_eq:
+  ∀x y.
+    x ≠ Diverge ∧ y ≠ Diverge ⇒
+    ((∀path. v_cmp path x y) ⇒ (getNum x) = (getNum y))
+Proof
+  rw []
+  \\ first_x_assum (qspec_then ‘[]’ assume_tac)
+  \\ Cases_on ‘x’
+  \\ fs [v_cmp_def,v_lookup_def,ltree_CASE]
+  \\ first_assum imp_res_tac
+  \\ Cases_on ‘y’
+  \\ fs [ltree_CASE]
+  \\ rw []
+  \\ imp_res_tac getNum_eq_same_length_args
+  \\ rw [] 
+QED
+
+(*maybe needed later.*)
+Triviality eval_strict_op_not_num_error:
+  ∀ x y .  x ≠ Diverge ∧
+           y ≠ Diverge ∧
+           ( (∀ n . x ≠ Num n) ∨ (∀ n. y ≠ Num n) )
+             ⇒ eval_op Add [x;y] = Error
+Proof
+  rw []
+  THEN1 (*(∀ n . x ≠ Num n) case *)(
+  rw [eval_op_def,getNum_def]
+  \\ Cases_on ‘x’ \\ rw [ltree_CASE,llist_CASES,getNum_def]
+  \\ rpt(   Cases_on ‘a’ \\ rw [ltree_CASE,llist_CASES,getNum_def]
+         \\ Cases_on ‘ts’ \\ rw [ltree_CASE,llist_CASES,getNum_def])
+  )(*(∀ n . y ≠ Num n) case *)
+  \\ Cases_on ‘∀ n . x ≠ Num n’ \\ fs []
+  THEN1 ((*(∀ n . x ≠ Num n) case, again *)
+  rw [eval_op_def]
+  \\ Cases_on ‘x’ \\ rw [ltree_CASE,llist_CASES,getNum_def]
+  \\ rpt(   Cases_on ‘a’ \\ rw [ltree_CASE,llist_CASES,getNum_def]
+         \\ Cases_on ‘ts’ \\ rw [ltree_CASE,llist_CASES,getNum_def])
+  ) THEN1 ( (*∀ n . y ≠ Num n ∧ x = Num n1 *)
+  rw [eval_op_def]
+  \\ Cases_on ‘y’ \\ rw [ltree_CASE,llist_CASES,getNum_def]
+  \\ rpt (   Cases_on ‘a’ \\ rw [ltree_CASE,llist_CASES,getNum_def]
+          \\ Cases_on ‘ts’ \\ rw [ltree_CASE,llist_CASES,getNum_def])
+  )
+QED
+
 Theorem eval_op_div:
   ∀op xs ys path.
     LIST_REL (λx y. ∀path. v_cmp path x y) xs ys ⇒
@@ -397,25 +462,28 @@ Theorem eval_op_div:
 Proof
   ho_match_mp_tac eval_op_ind \\ rw []
   \\ TRY (fs [eval_op_def] \\ rw [] \\ fs [v_cmp_refl] \\ NO_TAC)
-  THEN1
+  THEN1 (*op = Cons s *)
    (fs [eval_op_def] \\ fs [v_cmp_def]
     \\ Cases_on ‘path’ \\ fs [v_lookup_def]
     \\ imp_res_tac LIST_REL_LENGTH \\ fs [LNTH_fromList]
     \\ rw [] \\ fs [LIST_REL_EL_EQN])
-  THEN1
+  THEN1 (*op = If *)
    (fs [eval_op_def]
     \\ Cases_on ‘x1 = Diverge’ \\ fs []
     \\ qspec_then ‘Num' 0’ assume_tac v_cmp_LNIL_IMP
     \\ qspec_then ‘Num' 1’ assume_tac v_cmp_LNIL_IMP
     \\ fs []
-    \\ IF_CASES_TAC THEN1 (rw [] \\ imp_res_tac v_cmp_LNIL_IMP \\ fs [])
-    \\ IF_CASES_TAC THEN1 (rw [] \\ imp_res_tac v_cmp_LNIL_IMP \\ fs [])
+    \\ IF_CASES_TAC (*case x = 1 *)
+       THEN1 (rw [] \\ imp_res_tac v_cmp_LNIL_IMP \\ fs [])
+    \\ IF_CASES_TAC (*case x = 2 *)
+       THEN1 (rw [] \\ imp_res_tac v_cmp_LNIL_IMP \\ fs [])
+    (*case x ≠ 1 ∧ x ≠ 2 (Error) *)
     \\ Cases_on ‘y’ \\ fs []
     \\ Cases_on ‘ts’ \\ fs []
     \\ last_x_assum (qspec_then ‘[]’ mp_tac)
     \\ simp [Once v_cmp_def,v_lookup_def]
     \\ Cases_on ‘x1’ \\ fs [])
-  THEN1
+  THEN1 (*op = IsEq s *)
    (fs [eval_op_def]
     \\ Cases_on ‘x = Diverge’ \\ fs []
     \\ TRY (first_x_assum (qspec_then ‘[]’ mp_tac))
@@ -425,25 +493,37 @@ Proof
     \\ Cases_on ‘x’ \\ fs []
     \\ Cases_on ‘a’ \\ fs []
     \\ Cases_on ‘a’ \\ fs [])
-  \\ fs [eval_op_def,el_def]
-  \\ Cases_on ‘x = Diverge’ \\ fs []
-  \\ imp_res_tac v_cmp_Diverge2 \\ fs []
-  \\ Cases_on ‘x’ \\ Cases_on ‘y’ \\ simp []
-  \\ ‘a' = a ∧ LLENGTH ts' = LLENGTH ts’ by
-   (first_x_assum (qspec_then ‘[]’ mp_tac)
-    \\ fs [v_cmp_def,v_lookup_def])
-  \\ pop_assum mp_tac \\ simp []
-  \\ pop_assum mp_tac \\ simp []
-  \\ Cases_on ‘a’ \\ simp []
-  \\ strip_tac \\ strip_tac
-  \\ first_x_assum (qspec_then ‘i::path’ mp_tac)
-  \\ simp [v_lookup_def,v_cmp_def]
-  \\ pop_assum mp_tac \\ simp []
-  \\ rpt (pop_assum kall_tac)
-  \\ qspec_then ‘ts’ mp_tac fromList_fromSeq
-  \\ qspec_then ‘ts'’ mp_tac fromList_fromSeq
-  \\ rw [] \\ fs [LNTH_fromList]
-  \\ rfs [] \\ rw [] \\ fs []
+  THEN1 (*op = Proj s i*)
+   (fs [eval_op_def,el_def]
+    \\ Cases_on ‘x = Diverge’ \\ fs []
+    \\ imp_res_tac v_cmp_Diverge2 \\ fs []
+    \\ Cases_on ‘x’ \\ Cases_on ‘y’ \\ simp []
+    \\ ‘a' = a ∧ LLENGTH ts' = LLENGTH ts’ by
+      (first_x_assum (qspec_then ‘[]’ mp_tac)
+       \\ fs [v_cmp_def,v_lookup_def])
+    \\ pop_assum mp_tac \\ simp []
+    \\ pop_assum mp_tac \\ simp []
+    \\ Cases_on ‘a’ \\ simp []
+    \\ strip_tac \\ strip_tac
+    \\ first_x_assum (qspec_then ‘i::path’ mp_tac)
+    \\ simp [v_lookup_def,v_cmp_def]
+    \\ pop_assum mp_tac \\ simp []
+    \\ rpt (pop_assum kall_tac)
+    \\ qspec_then ‘ts’ mp_tac fromList_fromSeq
+    \\ qspec_then ‘ts'’ mp_tac fromList_fromSeq
+    \\ rw [] \\ fs [LNTH_fromList]
+    \\ rfs [] \\ rw [] \\ fs []   )
+  THEN1 (*op = Add *)
+   (fs []
+    \\ Cases_on ‘a1 = Diverge’ THEN1 (fs [eval_op_def])
+    \\ Cases_on ‘a2 = Diverge’ THEN1 (fs [eval_op_def])
+    \\ ‘y  ≠ Diverge’ by (imp_res_tac v_cmp_Diverge2)
+    \\ ‘y' ≠ Diverge’ by (imp_res_tac v_cmp_Diverge2)
+    \\ qspec_then ‘a1’ (qspec_then ‘y’ assume_tac) v_cmp_getNum_eq
+       \\ first_x_assum imp_res_tac 
+    \\ qspec_then ‘a2’ (qspec_then ‘y'’ assume_tac) v_cmp_getNum_eq
+       \\ first_x_assum imp_res_tac     
+    \\ fs [eval_op_def])
 QED
 
 Theorem eval_to_res_mono_lemma:
@@ -532,6 +612,20 @@ Proof
   \\ disch_then drule \\ fs []
 QED
 
+Theorem eval_to_not_diverge_mono:
+  ∀ k' k x . (k ≤ k' ∧ eval_to k x ≠ Diverge) ⇒ eval_to k' x ≠ Diverge
+Proof
+  rw []
+  \\ Cases_on ‘eval_to k x’ \\ Cases_on ‘eval_to k' x’ 
+  \\ qspecl_then
+        [‘x’,‘ts'’,‘ts’,‘k'’,‘k’,‘a'’,‘a’]
+        assume_tac (GEN_ALL eval_to_res_mono) \\ fs []
+  \\ first_assum imp_res_tac \\ rw []
+  \\ ‘eval_to k x ≠ Diverge’ by (fs [])
+  \\ ‘a' = a ∧ LLENGTH ts' = LLENGTH ts’ by (fs [])
+  \\ Cases_on ‘a’ \\ Cases_on ‘ts’ \\ Cases_on ‘ts'’ \\ fs []
+QED
+        
 Theorem dest_Closure_eval_IMP:
   dest_Closure (eval x) = NONE ⇒
   dest_Closure (eval_to k x) = NONE
@@ -863,6 +957,156 @@ Proof
   \\ metis_tac [eval_to_simple_mono]
 QED
 
+Theorem getNum_NONE:
+  (getNum x = NONE) = ∀n. x ≠ Num n
+Proof
+  Cases_on ‘x’
+  \\ Cases_on ‘a’ \\ Cases_on ‘ts’ \\ fs [getNum_def]
+QED
+
+Theorem getNum_SOME:
+  getNum x = SOME n ⇔ x = Num n
+Proof
+  Cases_on ‘x’
+  \\ Cases_on ‘a’ \\ Cases_on ‘ts’ \\ fs [getNum_def]
+QED
+
+Theorem eval_to_no_div_not_equal:
+  (k ≤ k')                    ∧
+  (eval_to k x ≠ Diverge)     ∧
+  (∀ n . eval_to k x ≠ Num n) ∧
+  (eval_to k' x ≠ Diverge)
+  ⇒ (∀ n . eval_to k' x ≠ Num n)
+Proof
+  rw []        
+  \\ Cases_on ‘eval_to k x’ \\ Cases_on ‘eval_to k' x’
+  \\ ‘eval_to k x ≠ Diverge’ by (fs [])
+  \\ qspecl_then [‘k'’,‘ts'’,‘a'’] assume_tac (Q.GENL [‘k1’,‘ts1’,‘a1’] eval_to_res_mono)
+  \\ first_x_assum imp_res_tac
+  \\ first_x_assum (qspec_then ‘n:num’ assume_tac)
+  \\ ‘a' = a
+      ∧ LLENGTH ts' = LLENGTH ts
+      ∧ Branch a ts ≠ Num n
+      ⇒ Branch a' ts' ≠ Num n’ by
+      (rw [] \\ fs [] \\ CCONTR_TAC \\ fs [])
+  \\ first_x_assum imp_res_tac \\ fs []
+QED
+
+(*potentially, this can be generalized from Num n to Branch a LNIL*)
+Theorem eval_to_forall_exists_swap:
+  (∀n. ∃k. eval_to k x ≠ Num n ∧ eval_to k x ≠ Diverge)
+       ⇒ (∃k. (∀n. eval_to k x ≠ Num n) ∧ eval_to k x ≠ Diverge)
+Proof
+  rw []
+  \\ first_assum (qspec_then ‘n’ assume_tac) \\ fs []
+  \\ qexists_tac ‘k’
+  \\ CONJ_TAC 
+  THEN1
+    (  pop_assum kall_tac
+    \\ pop_assum kall_tac
+    \\ CCONTR_TAC \\ fs []
+    \\ last_x_assum (qspec_then ‘n’ assume_tac) \\ fs []
+    \\ ‘eval_to k x ≠ Diverge’ by (fs [])
+    \\ Cases_on ‘eval_to k x’ \\ Cases_on ‘ts ≠ LNIL’ \\ fs []
+    \\ Cases_on ‘k≤k'’
+    THEN1 (qspec_then ‘k'’ imp_res_tac $ Q.GEN ‘k1’ eval_to_res_mono_LNIL \\ fs [])
+    \\ first_x_assum (fn t => ‘k' ≤ k’ by fs [t])
+    \\ qspecl_then [‘k’,‘k'’] imp_res_tac $ Q.GENL [‘k1’,‘k’] eval_to_simple_mono
+    \\ fs [])
+  \\ fs []
+QED
+        
+Theorem eval_Add:
+  eval (Prim Add [a1;a2]) =
+    (if eval a1 = Diverge then Diverge else
+     if eval a2 = Diverge then Diverge else
+       case (getNum (eval a1),getNum (eval a2)) of
+         | (SOME n1,SOME n2) => (Num (n1 + n2))
+         | _                 => Error
+    )
+Proof
+    fs [eval_def,eval_to_def,eval_op_def]
+  \\ IF_CASES_TAC \\ fs [gen_ltree_LNIL]
+  THEN1 (fs [v_limit_SOME] \\ qexists_tac ‘k’ \\ fs [])
+  \\ IF_CASES_TAC \\ fs [gen_ltree_LNIL]
+  THEN1
+   (fs [v_limit_SOME]
+   \\ qexists_tac ‘k’ \\ fs [])
+  \\ BasicProvers.TOP_CASE_TAC
+  THEN1
+   (fs [gen_ltree_LNIL,v_limit_SOME,getNum_NONE]
+    \\ last_x_assum (qspec_then ‘0’ strip_assume_tac) 
+    \\ last_x_assum (qspec_then ‘0’ strip_assume_tac)
+    \\ qexists_tac ‘MAX k' k''’
+    \\ rpt (strip_tac)
+    \\ rename [‘MAX k1 k2 ≤ k3’]
+    \\ IF_CASES_TAC
+    THEN1 (drule eval_to_div \\ fs[] \\ qexists_tac ‘k1’ \\ fs[])
+    \\ IF_CASES_TAC
+    THEN1 (drule eval_to_div \\ fs[] \\ qexists_tac ‘k2’ \\ fs[])
+    \\ pop_assum kall_tac
+    \\ drule eval_to_res_mono
+    \\ Cases_on ‘eval_to k3 a1’ \\ qpat_x_assum ‘_≠_’ kall_tac
+    \\ fs []
+    \\ Cases_on ‘a’ \\ fs [getNum_def]
+    \\ last_x_assum (qspecl_then [‘n’,‘k3’] strip_assume_tac)
+    \\ Cases_on ‘eval_to k' a1’
+    \\ disch_then drule \\ fs [] \\  rw []
+    \\ Cases_on ‘ts’ \\ Cases_on ‘ts'’ \\ fs [getNum_def])
+  \\ BasicProvers.TOP_CASE_TAC
+  THEN1
+   (fs [getNum_NONE,getNum_SOME,gen_ltree_LNIL,v_limit_SOME]
+    \\ ‘∀n. ∃k. eval_to k a2 ≠ Num n ∧ eval_to k a2 ≠ Diverge’ by
+      (fs [] \\ strip_tac
+       \\ first_x_assum (qspec_then ‘n’ assume_tac)
+       \\ last_x_assum kall_tac
+       \\ last_x_assum (qspec_then ‘0’ assume_tac) \\ fs []
+       \\ last_x_assum kall_tac
+       \\ first_x_assum (qspec_then ‘k'’ assume_tac) \\ fs []
+       \\ qspecl_then [‘k''’,‘k'’,‘a2’] imp_res_tac eval_to_not_diverge_mono 
+       \\ qexists_tac ‘k''’ \\ fs []
+      )
+    \\ qspec_then ‘a2’ imp_res_tac (Q.GEN ‘x’ eval_to_forall_exists_swap)
+    \\ last_x_assum (qspec_then ‘0’ strip_assume_tac)
+    \\ last_x_assum (qspec_then ‘0’ strip_assume_tac)
+    \\ last_x_assum kall_tac 
+    \\ last_x_assum kall_tac
+    \\ last_x_assum kall_tac
+    \\ qexists_tac ‘MAX (MAX k' k'') k'''’
+    \\ rpt (strip_tac)
+    \\ rename [‘MAX (MAX k1 k2) k3 ≤ k4’] \\ fs []
+    \\ qspecl_then [‘k4’,‘k2’,‘a1’] assume_tac eval_to_not_diverge_mono
+    \\ first_x_assum imp_res_tac
+    \\ qspecl_then [‘k4’,‘k3’,‘a2’] assume_tac eval_to_not_diverge_mono
+    \\ first_x_assum imp_res_tac
+    \\ fs [] \\ rw []
+    \\ Cases_on ‘getNum (eval_to k4 a1)’ \\ fs [getNum_SOME]
+    \\ ‘∀n. eval_to k4 a2 ≠ Num n’ by (
+      qspecl_then [‘a2’,‘k4’,‘k1’] imp_res_tac (GEN_ALL eval_to_no_div_not_equal))
+    \\ Cases_on ‘getNum (eval_to k4 a2)’ \\ fs [getNum_SOME])
+  \\ fs [getNum_NONE,getNum_SOME,gen_ltree_LNIL,v_limit_SOME]
+  \\ last_x_assum (qspec_then ‘k’ strip_assume_tac)
+  \\ last_x_assum (qspec_then ‘k'’ strip_assume_tac)
+  \\ last_x_assum (qspec_then ‘k'' ’ strip_assume_tac)
+  \\ last_x_assum (qspec_then ‘k'''’ strip_assume_tac)
+  \\ qpat_x_assum ‘_⇒_’ imp_res_tac
+  \\ qpat_x_assum ‘_⇒_’ imp_res_tac
+  \\ qexists_tac ‘MAX k'' k'''’
+  \\ rpt (strip_tac)
+  \\ rename [‘MAX k2 k3 ≤ k4’] \\ fs []
+  (*  eval_to k2 a1 = Num x ⇒ eval_to k4 a1 = Num x   *)
+  \\ Cases_on ‘eval_to k2 a1’ \\ Cases_on ‘ts’ \\ fs []
+  \\ ‘eval_to k2 a1 ≠ Diverge’ by (fs[])
+  \\ qspecl_then [‘a1’,‘k4’,‘k2’,‘a’] assume_tac (GEN_ALL eval_to_res_mono_LNIL)
+  \\ first_x_assum imp_res_tac
+  (*  eval_to k3 a2 = Num x' ⇒ eval_to k4 a2 = Num x'   *)
+  \\ Cases_on ‘eval_to k3 a2’ \\ Cases_on ‘ts’ \\ fs []
+  \\ ‘eval_to k3 a2 ≠ Diverge’ by (fs[])
+  \\ qspecl_then [‘a2’,‘k4’,‘k3’,‘a'’] assume_tac (GEN_ALL eval_to_res_mono_LNIL)
+  \\ first_x_assum imp_res_tac
+  \\ fs [getNum_def,getNum_SOME]                      
+QED
+                
 Theorem eval_Prim:
   eval (Prim op xs) = eval_op op (MAP eval xs)
 Proof
@@ -898,6 +1142,22 @@ Proof
     \\ fs [eval_def,eval_to_def,Once gen_ltree,eval_op_def]
     \\ fs [v_limit_def,v_lookup_def])
   \\ Cases_on ‘op’ \\ fs []
+  THEN1(
+  Cases_on ‘∃ x y . xs = [x;y]’
+   THEN1(
+       rw []
+       \\ simp [eval_Add]
+       \\ Cases_on ‘eval a1 = Diverge’ \\ fs [eval_op_def]
+    )THEN1(
+       fs []
+       \\ Cases_on ‘xs’ \\ fs [eval_def,eval_to_def,Once gen_ltree,eval_op_def]
+       \\ fs [v_limit_def,v_lookup_def]
+       \\ Cases_on ‘t’  \\ fs [eval_def,eval_to_def,Once gen_ltree,eval_op_def]
+       \\ fs [v_limit_def,v_lookup_def]
+       \\ Cases_on ‘t'’ \\ fs [eval_def,eval_to_def,Once gen_ltree,eval_op_def]
+       \\ fs [v_limit_def,v_lookup_def]
+    )
+  )
 QED
 
 Theorem eval_core:
